\begin{proof}[Proof of \cref{ThmA}]
\label{proofofA}
From \cref{traceofres} together with \cref{residytermvisjmfr} we get that 
\begin{multline}
\label{sum with alpha}
    r(\tr (d\phi u_n)) = \\
    (2\pi i )^n \1_{\{0\}}\left(\sum_{k=1}^r \sum_{|\alpha|=n-1} (n-1)!(\alpha_k + 1) dd^c \log | f_k |^2\wedge  (dd^c \log | f |^2)^{\alpha}\right).
\end{multline}
Let $v_k \in \N^r$ be the unit vector with a $1$ in the $k$:th position.  We rewrite the sum in \eqref{sum with alpha}
\begin{multline}
\label{pascals triangel 1}
    \sum_{k=1}^r \sum_{|\alpha|=n-1} \binom{n-1}{\alpha} (\alpha+v_k)!(dd^c \log | f |^2)^{\alpha+v_k} =  \\
    \sum_{|\beta|=n} \sum_{k=1}^r \binom{n-1}{\beta-v_k} \beta! (dd^c \log | f |^2)^{\beta}.
\end{multline}
The sum over $k$ is then calculated to 
\begin{equation}
\label{pascals triangel 2}
\sum_{k=1}^r \binom{n-1}{\beta-v_k} \beta! = \binom{n}{\beta} \beta! = n!
\end{equation}
as the coefficient  of $(dd^c \log |f|^2)^{\beta}$.
Finally, we see that the right hand side of \eqref{sum with alpha} can be written
\begin{equation}
    (2\pi i )^n n! \sum_{|\beta|=n} \1_{\{0\}}(dd^c \log | f |^2)^{\beta}
\end{equation}
which is precisely what we wanted to prove.
\end{proof}